GreedyDeriv/Examples.lean
@@ -26,55 +26,37 @@ def String.characterClass (s : String) : BA Char :=
 def r : Regex (BA Char) := plus 'a' "ab"
 #eval r.rmatch "ab".toList
 #eval r.gmatch "ab".toList
-
-example : Matches r (['a'], ['b']) := by
-  apply Matches.plus_left
-  apply Matches.pred
-  rfl
+#eval r.llmatch "ab".toList
 
 -- (a + ab)*
 def r2 : Regex (BA Char) := (plus 'a' "ab").star false
 #eval r2.rmatch "aab".toList
 #eval r2.gmatch "aab".toList
-
-example : Matches r2 (['a', 'a'], ['b']) := by
-  apply Matches.stars ['a'] ['a'] ['b']
-  apply Matches.plus_left
-  apply Matches.pred
-  rfl
-  apply Matches.stars ['a'] []
-  apply Matches.plus_left
-  apply Matches.pred
-  rfl
-  apply Matches.star_nil
+#eval r2.llmatch "aab".toList
 
 -- c + ab
 def r3 : Regex (BA Char) := plus 'c' (mul 'a' 'b')
 #eval r3.rmatch "ab".toList
 #eval r3.gmatch "ab".toList
-
-example : Matches r3 (['b', 'a'], []) := by
-  apply Matches.plus_right
-  apply Matches.mul ['a'] ['b'] []
-  apply Matches.pred
-  rfl
-  apply Matches.pred
-  rfl
+#eval r3.llmatch "ab".toList
 
 -- (a + aa)a
 def r4 : Regex (BA Char) := (plus 'a' "aa").mul 'a'
 #eval r4.rmatch "aaa".toList
 #eval r4.gmatch "aaa".toList
+#eval r4.llmatch "aaa".toList
 
 -- a*a
 def r5 : Regex (BA Char) := (star 'a' false).mul 'a'
 #eval r5.rmatch "aa".toList
 #eval r5.gmatch "aa".toList
+#eval r5.llmatch "aa".toList
 
 -- (ε|b)*
 def r6 : Regex (BA Char) := (epsilon.plus 'b').star false
 #eval r6.rmatch "bb".toList
 #eval r6.gmatch "bb".toList
+#eval r6.llmatch "bb".toList
 
 -- (ε|b)(ε|b)*
 def r6' : Regex (BA Char) := (epsilon.plus 'b').mul ((epsilon.plus 'b').star false)
@@ -85,43 +67,70 @@ def r6' : Regex (BA Char) := (epsilon.plus 'b').mul ((epsilon.plus 'b').star fal
 def r7 : Regex (BA Char) := (plus 'a' (epsilon.plus 'b')).star false
 #eval r7.rmatch "aaaabbb".toList
 #eval r7.gmatch "aaaabbb".toList
+#eval r7.llmatch "aaaabbb".toList
 
 -- (ε|a)b
 def r8 : Regex (BA Char) := (epsilon.plus 'a').mul 'b'
 #eval r8.rmatch "ab".toList
 #eval r8.gmatch "ab".toList
+#eval r8.llmatch "ab".toList
 
 -- ((a|ε|b)|b)
 def r9 : Regex (BA Char) := Regex.plus ((plus 'a' epsilon).plus 'b') 'b'
 #eval r9.gmatch "b".toList
 #eval r9.rmatch "b".toList
+#eval r9.llmatch "b".toList
 
 -- (ε|a)*b
 def r10 : Regex (BA Char) := ((Regex.plus epsilon 'a').star false).mul 'b'
 #eval r10.gmatch "ab".toList
 #eval r10.rmatch "ab".toList
+#eval r10.llmatch "ab".toList
 
 -- (a|ε)*(ε|b)
 def r11 : Regex (BA Char) := ((Regex.plus 'a' epsilon).star false).mul (Regex.plus (epsilon) 'b')
 #eval r11.gmatch "ab".toList
 #eval r11.rmatch "ab".toList
+#eval r11.llmatch "ab".toList
 
 -- (ε|a)*(ε|b)
 def r12 : Regex (BA Char) := ((Regex.plus epsilon 'a').star false).mul (Regex.plus (epsilon) 'b')
 #eval r12.gmatch "ab".toList
 #eval r12.rmatch "ab".toList
+#eval r12.llmatch "ab".toList
 
 -- (a|ε|b)*b
 def r13 : Regex (BA Char) := ((Regex.plus 'a' (Regex.plus epsilon 'b')).star false).mul 'b'
 #eval r13.gmatch "bb".toList
 #eval r13.rmatch "bb".toList
+#eval r13.llmatch "bb".toList
 
 -- a*?a
 def r14 : Regex (BA Char) := (star 'a' true).mul 'a'
 #eval r14.rmatch "aaa".toList
 #eval r14.gmatch "aaa".toList
+#eval r14.llmatch "aaa".toList
 
 -- a*?b
 def r15 : Regex (BA Char) := (star 'a' true).mul 'b'
 #eval r15.rmatch "aab".toList
 #eval r15.gmatch "aab".toList
+#eval r15.llmatch "aab".toList
+
+-- a + aa
+def r16 : Regex (BA Char) := (plus 'a' "aa").star false
+#eval r16.rmatch "aa".toList
+#eval r16.gmatch "aa".toList
+#eval r16.llmatch "aa".toList
+
+-- (a + aa)b
+def r17 : Regex (BA Char) := (plus 'a' "ab").mul 'b'
+#eval r17.rmatch "abb".toList
+#eval r17.gmatch "abb".toList
+#eval r17.llmatch "abb".toList
+
+-- (a + aa)aa
+def r18 : Regex (BA Char) := (plus 'a' "aa").mul "aa"
+#eval r18.rmatch "aaa".toList
+#eval r18.gmatch "aaa".toList
+#eval r18.llmatch "aaa".toList
